.

casestudy/openSSL/pmac_verify_hmac/pmac_verify_hmac_proof_BL_CL32.ec
@@ -1,21 +1,71 @@
-require import AllCore IntDiv CoreMap List.
 from Jasmin require import JModel Leakage_models.
-require Pmac_verify_hmac_ct.
+require import AllCore IntDiv CoreMap List Pmac_verify_hmac_ct.
+
 import StdOrder.IntOrder Ring.IntID.
 
-clone import Pmac_verify_hmac_ct.T with
-theory LeakageModel <-  LeakageModelCL32.
+clone import Pmac_verify_hmac_ct.T with theory LeakageModel <-  LeakageModelCL32.
+
+lemma invwK (c:W64.t) : invw (invw c) = c.
+proof. by apply W64.wordP => i hi; rewrite !W64.invwE hi. qed.
+
+lemma sar_and (x y:W64.t): W64.sar x 63 `&` y = if to_sint x < 0 then y else W64.zero.
+proof.
+  apply W64.wordP => i hi.
+  rewrite W64.andwE /sar W64.initiE 1:// /=.
+  have -> : min 63 (i + 63) = 63 by smt().
+  rewrite to_sintE /smod W64.get_to_uint /=.
+  have /= := W64.to_uint_cmp x; smt (W64.zerowE).
+qed.
+
+op inv (j off i:W64.t) = 
+   if to_uint j < to_uint off then to_uint i = 0
+  else if to_uint j < to_uint off + 20 then to_uint i = to_uint j - to_uint off
+  else to_uint i = 20.
+
+lemma inv_incr j off i : 
+  W64.to_uint j < 276 => 
+  inv j off i =>
+  inv (j + W64.one) off
+    (i + invw (invw (j - off - W64.of_int 20 `|>>` W8.of_int 63)) `&` (off - W64.one - j `|>>` W8.of_int 63) `&` W64.one).
+proof.
+  rewrite !invwK /W64.(`|>>`) W8.to_uint_small 1:// modz_small 1://.
+  rewrite !sar_and /inv => /> hj.
+  rewrite (W64.to_uintD_small j W64.one) 1:/#.
+  have -> : to_sint (j - off - W64.of_int 20) = to_uint j - to_uint off - 20.
+  + admit.
+  have heq : to_sint (off - W64.one - j) = to_uint off - 1 - to_uint j.
+  + admit.
+  case: (to_uint j < to_uint off) => hjoff /=.
+  + move=> hi; have -> /= : to_uint j - to_uint off - 20 < 0 by smt().
+    by rewrite sar_and heq; have -> /= /#: !(to_uint off - 1 - to_uint j < 0) by smt().
+  case: (to_uint j < to_uint off + 20) => hjoff20.
+  + have -> /= :  to_uint j - to_uint off - 20 < 0 by smt().
+    rewrite sar_and heq => hi.
+    split => hj1.
+    + by have -> /= : !(to_uint off - 1 - to_uint j < 0); smt().
+    case: (to_uint off - 1 - to_uint j < 0) => hoff1j /=.
+    + by rewrite (W64.to_uintD_small i W64.one) /= /#.
+    smt().    
+  have -> /= : !(to_uint j - to_uint off - 20 < 0); smt().
+qed.
 
 equiv l_final : M.verify_hmac_jazz ~ M.verify_hmac_jazz :
-={M.leakages, len, pmac, out, maxpad} /\
-  to_uint pmac{2} + 32 <= W64.modulus /\
-  32 %| to_uint pmac{2}
-==> ={M.leakages}.
+  ={M.leakages, len, pmac, out, maxpad} /\ to_uint pmac{2} + 32 <= W64.modulus /\ 32 %| to_uint pmac{2} /\ to_uint maxpad{1} < 256 
+  ==> ={M.leakages}.
 proof.
-proc; inline *; auto.
-while (={maxpad, j, p, M.leakages, len, pmac, out, maxpad} /\ to_uint pmac{2} + 32 <= W64.modulus
-        /\ 32 %| to_uint pmac{2}).
-wp; skip=> />.
-+ move=> &1 &2 /= hpmac hdiv32 ht.
-  rewrite /leak_mem /= /leak_mem_CL32 /=. rewrite !offset_div_32.
-admitted.
+proc; wp => /=.
+while (={maxpad, j, p, M.leakages, len, pmac, out, maxpad} /\ 
+       inv j{1} off{1} i{1} /\ inv j{2} off{2} i{2} /\ to_uint j{1} <= to_uint maxpad{1} < 256 + 20 /\ 
+       to_uint pmac{2} + 32 <= W64.modulus /\ 32 %| to_uint pmac{2}).
++ wp; skip=> |> &1 &2 h1 h2 hjm hmax hpmac dpmac; rewrite ultE => hj.
+  split.
+  + by rewrite /leak_mem /leak_mem_CL32 !offset_div_32 // 1,2:/#.
+  split; 1: by apply inv_incr => //; smt().
+  split; 1: by apply inv_incr => //; smt().
+  by rewrite (W64.to_uintD_small j{2} W64.one) /#.
+auto => |> &2 hmac dmac hmax.
+rewrite (W64.to_uintD_small maxpad{2}) /= 1:/#.
+have -> : out{2} - (out{2} + len{2} - W64.one - maxpad{2} - W64.of_int 20) = 
+          (W64.one + maxpad{2} + W64.of_int 20) - len{2} by ring.
+rewrite /inv /=; smt(W64.to_uint_cmp).
+qed.
